p4light value helpers & clean up

deps/poulet4/lib/AList.v
@@ -2,7 +2,7 @@ Require Import Coq.Classes.EquivDec.
 Require Import Coq.Lists.List.
 Require Import Coq.Sorting.Permutation.
 Require Import Coq.Bool.Sumbool.
-Require Import Coq.Classes.Morphisms.
+Require Import Coq.Classes.Morphisms Poulet4.Utils.
 Import ListNotations.
 
 Definition AList
@@ -264,7 +264,11 @@ Section AList.
       key_unique l = true -> key_unique (filter l f) = true.
   Proof. intros. apply key_unique_sublist_true with l; auto. apply filter_sublist. Qed.
 
-  Inductive all_values {A B} (hold_one_value : A -> B -> Prop) :
+  Definition all_values {A B} (hold_one_value : A -> B -> Prop) :
+    AList K A R -> AList K B R -> Prop :=
+    Forall2 (fun a b => fst a = fst b /\ hold_one_value (snd a) (snd b)).
+  
+  (*Inductive all_values {A B} (hold_one_value : A -> B -> Prop) :
                        AList K A R -> AList K B R -> Prop :=
   | all_values_nil : all_values hold_one_value nil nil
   | all_values_cons : forall k v v' kvs kvs',
@@ -272,7 +276,7 @@ Section AList.
                       all_values hold_one_value kvs kvs' ->
                       all_values hold_one_value ((k, v):: kvs) ((k, v'):: kvs').
 
-  Local Hint Constructors all_values : core.
+  Local Hint Constructors all_values : core.*)
   
   Lemma Forall2_all_values :
     forall (U W : Type) (P : U -> W -> Prop) us ws ks,
@@ -280,28 +284,26 @@ Section AList.
       Forall2 P us ws <->
       all_values P (combine ks us) (combine ks ws).
   Proof.
-    intros U W P us ws ks Hlku Hlkw; split.
-    - intro Hfa2; clear Hlku Hlkw.
-      generalize dependent ks.
-      induction Hfa2; intros [| k ks]; simpl in *; auto.
-    - intro Hav.
-      remember (combine ks us) as kus eqn:Heqkus;
-        remember (combine ks ws) as kws eqn:Heqkws;
-        generalize dependent ws;
-        generalize dependent us;
-        generalize dependent ks.
-      induction Hav;
-        intros [| ky ks] [| u us]
-               Hlkus Hus [| w ws] Hlkws Hws; simpl in *;
-          inversion Hus; inversion Hws;
-            inversion Hlkus; inversion Hlkws; subst; eauto.
+    intros U W P us ws ks Hlku Hlkw; unfold all_values.
+    rewrite Forall2_conj.
+    rewrite Forall2_map_both with (f := fst) (g := fst).
+    rewrite Forall2_map_both with (f := snd) (g := snd).
+    repeat rewrite map_snd_combine by auto.
+    repeat rewrite map_fst_combine by auto.
+    rewrite Forall2_Forall, Forall_forall.
+    intuition.
   Qed.
 
   Lemma all_values_keys_eq : forall {U W} (P : U -> W -> Prop) us ws,
       all_values P us ws -> map fst us = map fst ws.
   Proof.
     intros U W P us ws HPuws.
-    induction HPuws; simpl in *; f_equal; auto.
+    unfold all_values in HPuws.
+    rewrite Forall2_conj in HPuws.
+    destruct HPuws as [HPl _].
+    rewrite Forall2_map_both in HPl.
+    rewrite Forall2_eq in HPl.
+    assumption.
   Qed.
   
   Fixpoint map_values {A B} (f : A -> B) (l : AList K A R): AList K B R :=
